ArchSemTinyArm/PromisingFirstProof.lean
@@ -1,0 +1,151 @@
+import ArchSemTinyArm.Promising
+import ArchSem.TerminatingModel
+
+open ArchSemTinyArm.Promising
+open ArchSem.TerminatingModel
+open ArchSem.NondeterministicMonad
+
+
+-- TODO: I can probably simplify this by rearranging order of cases.
+theorem NExcept.bind_iff {ε α β} (b : β) (m : NExcept ε α) (f : α → NExcept ε β)
+     : b ∈ (NExcept.bind m f).oks ↔ ∃ (a : α), a ∈ m.oks ∧ b ∈ (f a).oks
+  := by
+  apply Iff.intro
+  case mp =>
+    intro h
+    simp [NExcept.bind] at h
+    revert h
+    induction m.oks
+    case nil =>
+      intro h
+      simp [List.map] at h
+    case cons tail ih =>
+      rename_i head
+      intro mem
+      simp [NExcept.merge] at mem
+      rcases mem
+      case inl =>
+        rename_i h
+        exact ⟨head, by simp, h⟩
+      case inr =>
+        rename_i h
+        have := ih h
+        rcases this with ⟨a, l, r⟩
+        exact ⟨a, List.Mem.tail _ l, r⟩
+  case mpr =>
+    intro h
+    simp [NExcept.bind]
+    revert h
+    induction m.oks
+    case nil =>
+      intro h
+      simp at h
+    case cons tail ih =>
+      intro h
+      rename_i head
+      rcases h with ⟨a, h⟩
+      rcases h with ⟨left, right⟩
+      rcases left
+      case head =>
+        simp [List.map, NExcept.merge]
+        apply Or.inl
+        exact right
+      case tail inTail =>
+        simp [List.map, NExcept.merge]
+        apply Or.inr
+        apply ih
+        exact ⟨a, inTail, right⟩
+
+theorem NEStateM.bind_iff {ε σ α β} (s₀ : σ) (s : σ) (b : β) (m : NEStateM ε σ α) (f : α → NEStateM ε σ β)
+    : (s, b) ∈ (NEStateM.bind m f s₀).oks ↔ ∃ (s' : σ) (a : α), (s', a) ∈ (m s₀).oks ∧ (s, b) ∈ (f a s').oks
+  := by
+  simp [Bind.bind, NEStateM.bind]
+  have base := @NExcept.bind_iff (σ × ε) (σ × α) (σ × β) (s, b) (m s₀) (fun p => f p.snd p.fst)
+  conv => lhs ; lhs ; rhs ; rhs ; intro p
+  conv at base => rhs ; simp
+  exact base
+
+section PromiseFirstProof
+
+variable (isem : SailM Unit) (nThreads : Nat) (termCond : TerminationCondition nThreads)
+
+theorem run_to_termination_monotonic_fuel
+    (promises : List Msg) (pstate : ProjectedModelState) (tid : Fin nThreads) (initmem : InitialMem) (mem : PromisingMemory)
+    (fuel : Nat)
+    : ∀ s ∈ (runToTermination tid initmem isem termination fuel base (promises, pstate)).oks,
+        s.snd →
+        s ∈ (runToTermination tid initmem isem termination (fuel + 1) base (promises, pstate)).oks
+  := by
+  induction fuel generalizing promises pstate with
+  | zero =>
+    simp [runToTermination]
+    intros
+    contradiction
+  | succ f ih =>
+    intro s mem fuelRemains
+    simp [runToTermination, Bind.bind] at mem
+    repeat rw [NEStateM.bind_iff] at mem
+    rcases mem with ⟨s', a', h_interp, h⟩
+    simp [get, NEStateM.bind, Bind.bind, pure, NExcept.pure, NExcept.bind, NExcept.merge, modify] at h
+    split at h
+    -- TODO: fix lots of repetition in the cases
+    case succ.isFalse =>
+      simp [modify, modifyGet, NEStateM.bind, bind, pure, NExcept.pure, NExcept.bind, NExcept.merge] at h
+      have := ih s'.fst { threadState := s'.snd.threadState, mem := s'.snd.mem, iis := IIS.init } s h fuelRemains
+      rw [runToTermination]
+      simp [Bind.bind]
+      repeat rw [NEStateM.bind_iff]
+      refine ⟨s', a', h_interp, ?_⟩
+      simp [get, NEStateM.bind, Bind.bind, pure, NExcept.pure, NExcept.bind, NExcept.merge, modify]
+      split
+      case isFalse =>
+        simp [modifyGet, NEStateM.bind, bind, pure, NExcept.pure, NExcept.bind, NExcept.merge]
+        exact this
+      case isTrue =>
+        contradiction
+    case succ.isTrue =>
+      rw [runToTermination]
+      simp [Bind.bind]
+      repeat rw [NEStateM.bind_iff]
+      refine ⟨s', a', h_interp, ?_⟩
+      simp [get, NEStateM.bind, Bind.bind, pure, NExcept.pure, NExcept.bind, NExcept.merge, modify]
+      split
+      case isFalse =>
+        contradiction
+      case isTrue =>
+        assumption
+
+theorem enumerate_result_promises_monotonic_fuel
+   : ∀ (ts : ThreadState) (initmem : InitialMem) (mem : PromisingMemory)
+       (tid : Fin nThreads) (fuel : Nat),
+     ∀ s ∈ (enumerateResults fuel tid initmem isem termCond ts mem).promises,
+       s ∈ (enumerateResults (fuel + 1) tid initmem isem termCond ts mem).promises
+ := by
+ sorry
+
+theorem promise_select_tid_monotonic_fuel
+   : ∀ (pState : ModelState nThreads) (tid : Fin nThreads) (fuel : Nat),
+     ∀ s ∈ (promiseSelectTid fuel pState tid isem termCond).oks,
+       s ∈ (promiseSelectTid (fuel + 1) pState tid isem termCond).oks
+ := by
+ sorry
+
+theorem run_step_monotonic_fuel
+   : ∀ (pState : ModelState nThreads) (fuel : Nat),
+     ∀ s ∈ (runStep fuel isem termCond pState).oks,
+       s ∈ (runStep (fuel + 1) isem termCond pState).oks
+ := by
+ sorry
+
+theorem naive_runtime_monotonic_fuel
+    : ∀ (pState : ModelState nThreads) (fuel : Nat),
+      ∀ r ∈ (runNaive fuel isem nThreads termCond pState).oks,
+        r ∈ (runNaive (fuel + 1) isem nThreads termCond pState).oks
+  := by
+  intro pState fuel r mem
+  simp [runNaive] at mem ⊢
+
+  simp [Bind.bind, NEStateM.bind] at ⊢
+  sorry
+
+end PromiseFirstProof
